2pc protocol with par cmd (#1014)
This PR accomplishes a proof of the 2pc protocol using a proof rule for
the parallel cmd for summarizing unbounded number of right mover voting
actions. The resulting proof is more succinct that previous attempts
based on pending asyncs. This proof also has the desirable property that
it works for arbitrary number of instance of 2pc potentially running
concurrently.

After this PR lands, this is the only proof of 2PC in the repository.

---------

Co-authored-by: Shaz Qadeer <shaz.qadeer@gmail.com>

Test/civl/async/2pc.bpl
@@ -1,444 +1,208 @@
 // RUN: %parallel-boogie "%s" > "%t"
 // RUN: %diff "%s.expect" "%t"
 
-// ###########################################################################
-// Type declarations
+/*
+2pc protocol: 
+A transaction needs to be executed at every replica. Every replica executes each step of the transaction
+but does not mark the transaction as complete until the coordinator runs the 2pc protocol to collectively
+decide whether to commit or abort the transaction.
 
-// Transaction and Machine IDs
-type Xid = int;
-type Mid = int;
+There are two phases in the protocol. In the first phase, the coordinator sends vote requests to all replicas.
+The replicas then send a reply (yes/no) to the coordinator. If all replies are yes, then the coordinator sends
+a commit decision to all replicas, otherwise it sends an abort decision. After receiving the decision from the
+coordinator, the transaction is marked as complete at each replica if it was a commit decision, or cancelled
+if it was an abort decision.
 
-const CoordinatorMid : Mid;
-axiom CoordinatorMid == 0;
-function coordinatorMid (mid : Mid) : bool { mid == CoordinatorMid }
+Model proved below:
+Let's say there are multiple transactions at each replica that are marked as incomplete. Then multiple instances
+of the coordinator may be running concurrently, each executing the 2pc protocol one transaction.
+The goal is to ensure that we don't ever commit conflicting transactions; this condition is used to
+abstractly model consistency of committed transactions.
+We model the conflict relation between transactions using a 2-d array Conflict with axioms.
 
-const numParticipants : int;
-axiom 0 < numParticipants;
-function participantMid (mid : Mid) : bool { 1 <= mid && mid <= numParticipants }
+Proof obligation:
+We have a ghost variable, committed_transactions, which keeps track of all transactions that have been committed so far.
+Before adding a transaction to this set, we assert that the transaction being added does not conflict with any previously
+committed transactions. If this assertion is shown to hold in all executions of the protocol, it should imply that
+we never commit conflicting transactions.
+*/
 
-datatype Pair { Pair(xid: Xid, mid: Mid) }
+type TransactionId;
+type ReplicaId = int;
 
-function {:inline} pair (xid: Xid, mid: Mid, p: Pair) : bool
-{ p == Pair(xid, mid) && participantMid(p->mid) }
+datatype Vote { YES(), NO(), NONE() }
+datatype VoteRequest { VoteRequest(xid: TransactionId, rid: ReplicaId) }
+datatype VoteRequestToken { VoteRequestToken(xid: TransactionId, rid: ReplicaId) }
+datatype Decision { COMMIT(), ABORT() }
 
-function {:inline} perm (xid: Xid) : Set Pair
-{ Set((lambda p: Pair :: pair(xid, p->mid, p))) }
+const Conflict: [TransactionId][TransactionId]bool;
+const n: int;
+axiom 0 < n;
+axiom (forall xid1: TransactionId, xid2: TransactionId :: Conflict[xid1][xid2] == Conflict[xid2][xid1]);
+axiom (forall xid0: TransactionId :: Conflict[xid0][xid0] == true);
 
-// Transaction State
-type MState = int;
-function {:inline} ABORTED   () : int { 0 }
-function {:inline} UNDECIDED () : int { 1 }
-function {:inline} COMMITTED () : int { 2 }
-function {:inline} Aborted   (i:MState) : bool { i == ABORTED() }
-function {:inline} Undecided (i:MState) : bool { i == UNDECIDED() }
-function {:inline} Committed (i:MState) : bool { i == COMMITTED() }
-function {:inline} UndecidedOrAborted   (i:MState) : bool { Undecided(i) || Aborted(i) }
-function {:inline} UndecidedOrCommitted (i:MState) : bool { Undecided(i) || Committed(i) }
+var {:layer 0,1} locked_transactions: [ReplicaId](Set TransactionId);
+var {:layer 0,1} committed_transactions: Set TransactionId;
 
-type XState = [Mid]MState;
-type GState = [Xid]XState;
-
-// ###########################################################################
-// Global shared variables
-
-var {:layer 0,11} state : GState;
-var {:layer 7,8} votes : [Xid]int;
-
-var {:linear} {:layer 7,9} B: Set Pair;
-var {:linear} {:layer 7,10} UnallocatedXids: Set Pair;
-
-// ###########################################################################
-// Consistency Predicates
-
-// Transaction (indicated by prefix x)
-
-function {:inline} xUndecided (state: XState) : bool
+function noConflicts(xids: (Set TransactionId), xid: TransactionId) : bool
 {
-  Undecided(state[CoordinatorMid]) &&
-  (forall i : Mid :: participantMid(i) ==> Undecided(state[i]))
+    !(exists x: TransactionId :: Set_Contains(xids, x) && Conflict[x][xid])
 }
 
-function {:inline} xUndecidedOrCommitted (state: XState) : bool
+function allVoteRequests(xid: TransactionId) : Set VoteRequest
 {
-  UndecidedOrCommitted(state[CoordinatorMid]) &&
-  (forall i : Mid :: participantMid(i) ==> UndecidedOrCommitted(state[i]))
+    Set((lambda vr:VoteRequest :: vr->xid == xid &&  1 <= vr->rid && vr->rid < n+1))
 }
 
-function {:inline} xUndecidedOrAborted (state: XState) : bool
+function remainingVoteRequests(xid: TransactionId, i:int) : Set VoteRequest
 {
-  UndecidedOrAborted(state[CoordinatorMid]) &&
-  (forall i : Mid :: participantMid(i) ==> UndecidedOrAborted(state[i]))
+    Set((lambda vr:VoteRequest :: vr->xid == xid &&  i <= vr->rid && vr->rid < n+1))
 }
 
-function {:inline} xConsistent (state: XState) : bool
+yield procedure {:layer 1} TPC({:linear} xid: One TransactionId, {:linear_in} vrs: (Set VoteRequest))
+requires {:layer 1} vrs == allVoteRequests(xid->val);
+requires call LockedNoConflicts();
+requires call CommittedSubsetLocked();
+requires call XidNotInCommitted(xid);
 {
-  xUndecidedOrCommitted(state) || xUndecidedOrAborted(state)
-}
+    var d: Decision;
+    var votes: [ReplicaId]Vote;
+    var {:linear} vrs': Set VoteRequest;
+    var i: int;
 
-function {:inline} xNoUndoneDecision (oldState: XState, newState: XState) : bool
-{
-  (newState[CoordinatorMid] == oldState[CoordinatorMid] || Undecided(oldState[CoordinatorMid])) &&
-  (forall i : Mid :: participantMid(i) ==> (newState[i] == oldState[i] || Undecided(oldState[i])))
-}
+    d := COMMIT();
+    vrs' := vrs;
 
-function {:inline} xConsistentExtension (oldState: XState, newState: XState) : bool
-{
-  xConsistent(newState) &&
-  xNoUndoneDecision(oldState, newState)
-}
-
-function {:inline} xAllParticipantsInB (xid: Xid, B: Set Pair) : bool
-{
-  (forall mid: Mid :: participantMid(mid) ==> Set_Contains(B, Pair(xid, mid)))
-}
-
-// Globally across transactions (indicated by prefix g)
-
-function {:inline} gUndecided (state: GState) : bool
-{
-  (forall j: Xid :: xUndecided(state[j]))
-}
-
-function {:inline} gConsistent (state: GState) : bool
-{
-  (forall j: Xid :: xConsistent(state[j]))
-}
-
-// Helper predicates
-
-function {:inline} ExistsMonotoneExtension (snapshot: GState, state: GState, xid: Xid) : bool
-{
-  (exists newState: XState ::
-    state == snapshot[xid := newState] && xNoUndoneDecision(snapshot[xid],newState))
-}
-
-function {:inline} VotesEqCoordinatorState (votes: [Xid]int, state: GState, xid: Xid) : bool
-{
-     ( (votes[xid] == -1)                                == Aborted  (state[xid][CoordinatorMid]) )
-  && ( (0 <= votes[xid] && votes[xid] < numParticipants) == Undecided(state[xid][CoordinatorMid]) )
-  && ( (votes[xid] == numParticipants)                   == Committed(state[xid][CoordinatorMid]) )
-}
-
-// ###########################################################################
-// Yield assertions
-
-function {:inline} SetInv (B: [Pair]bool) : bool
-{
-  (forall xid: Xid, mid: Mid :: B[Pair(xid,mid)] ==> participantMid(mid))
-}
-
-function {:inline} Inv_8 (state: GState, B: Set Pair, votes: [Xid]int) : bool
-{
-     gConsistent(state)
-  && SetInv(B->val)
-  && (forall xid: Xid :: VotesEqCoordinatorState(votes, state, xid))
-  && (forall xid: Xid :: votes[xid] == -1 || votes[xid] == card(B->val, xid))
-  && (forall p: Pair :: Set_Contains(B, p) && votes[p->xid] != -1 ==> UndecidedOrCommitted(state[p->xid][p->mid]))
-}
-
-function {:inline} Inv_9 (state: GState, B: Set Pair, xid: Xid) : bool
-{
-     gConsistent(state)
-  && (xAllParticipantsInB(xid, B) || xUndecidedOrAborted(state[xid]))
-}
-
-yield invariant {:layer 8} YieldInv_8 ();
-invariant Inv_8(state, B, votes);
-
-yield invariant {:layer 8} YieldUndecidedOrCommitted_8 (xid: Xid, mid: Mid, {:linear} pair: One Pair);
-invariant pair(xid, mid, pair->val) && (votes[xid] == -1 || UndecidedOrCommitted(state[xid][mid]));
-
-yield invariant {:layer 8} YieldAborted_8 (xid: Xid, mid: Mid, {:linear} pair: One Pair);
-invariant pair(xid, mid, pair->val) && Aborted(state[xid][mid]);
-
-yield invariant {:layer 9} YieldInv_9 (xid: Xid);
-invariant Inv_9(state, B, xid);
-
-yield invariant {:layer 9} YieldConsistent_9 ();
-invariant gConsistent(state);
-
-yield invariant {:layer 10} YieldConsistent_10 ();
-invariant gConsistent(state);
-
-// ###########################################################################
-// Main
-
-yield procedure {:layer 11}
-main ()
-requires call YieldInv_8();
-requires call YieldConsistent_9();
-requires call YieldConsistent_10();
-{
-  var xid: Xid;
-  while (*)
-  invariant {:yields} true;
-  invariant call YieldInv_8();
-  invariant call YieldConsistent_9();
-  invariant call YieldConsistent_10();
-  {
-    call xid := Coordinator_TransactionReq();
-  }
-}
-
-// ###########################################################################
-// Event Handlers
-
-atomic action {:layer 11} atomic_Coordinator_TransactionReq () returns (xid: Xid)
-modifies state;
-{
-  var {:pool "A"} x: XState;
-  state[xid] := x;
-  assume xConsistent(state[xid]);
-}
-
-yield procedure {:layer 10}
-Coordinator_TransactionReq () returns (xid: Xid)
-refines atomic_Coordinator_TransactionReq;
-preserves call YieldInv_8();
-preserves call YieldConsistent_9();
-preserves call YieldConsistent_10();
-{
-  var {:linear} pair: One Pair;
-  var {:linear} pairs: Set Pair;
-  var {:layer 10} snapshot: GState;
-  var i : Mid;
-
-  call xid, pairs := AllocateXid();
-  call {:layer 10} snapshot := Copy(state);
-  i := 1;
-  while (i <= numParticipants)
-  invariant {:layer 8} Inv_8(state, B, votes);
-  invariant {:layer 8,9,10} pairs == Set((lambda p: Pair :: pair(xid, p->mid, p) && i <= p->mid));
-  invariant {:layer 8} votes[xid] == -1 || (forall p: Pair :: Set_Contains(pairs, p) ==> UndecidedOrCommitted(state[xid][p->mid]));
-  invariant {:layer 9} Inv_9(state, B, xid);
-  invariant {:layer 10} gConsistent(state);
-  invariant {:layer 10} ExistsMonotoneExtension(snapshot, state, xid);
-  invariant {:layer 8,9,10} 1 <= i && i <= numParticipants + 1;
-  {
-    call pair := One_Get(pairs, Pair(xid, i));
-    async call {:sync} Participant_VoteReq(xid, i, pair);
-    i := i + 1;
-  }
-
-  assert {:layer 10} {:add_to_pool "A", state[xid]} true;
-}
-
-// ---------------------------------------------------------------------------
-
-left action {:layer 10} atomic_Participant_VoteReq (xid: Xid, mid: Mid, {:linear_in} pair: One Pair)
-modifies state;
-{
-  var {:pool "A"} next_state_xid: XState;
-  assert Set_IsDisjoint(perm(xid), UnallocatedXids);
-  assert pair(xid, mid, pair->val);
-  assert {:add_to_pool "A", state[xid]} xConsistent(state[xid]);
-  assume {:add_to_pool "A", next_state_xid} xConsistentExtension(state[xid], next_state_xid);
-  state[xid] := next_state_xid;
-}
-
-yield procedure {:layer 9}
-Participant_VoteReq (xid: Xid, mid: Mid, {:linear_in} pair: One Pair)
-refines atomic_Participant_VoteReq;
-requires call YieldInv_8();
-requires call YieldUndecidedOrCommitted_8(xid, mid, pair);
-requires call YieldInv_9(xid);
-{
-  if (*) {
-    async call {:sync} Coordinator_VoteYes(xid, mid, pair);
-  } else {
-    call SetParticipantAborted(xid, mid, pair);
-    async call {:sync} Coordinator_VoteNo(xid, mid, pair);
-  }
-
-  assume {:add_to_pool "A", state[xid]} true;
-}
-
-// ---------------------------------------------------------------------------
-
-left action {:layer 9} atomic_Coordinator_VoteYes (xid: Xid, mid: Mid, {:linear_in} pair: One Pair)
-modifies state, B;
-{
-  var {:pool "A"} next_state_xid: XState;
-  assert Set_IsDisjoint(perm(xid), UnallocatedXids);
-  assert pair(xid, mid, pair->val);
-  assert xConsistent(state[xid]);
-  call One_Put(B, pair);
-  if (*) {
-    assume {:add_to_pool "A", next_state_xid} xConsistentExtension(state[xid], next_state_xid);
-    state[xid] := next_state_xid;
-    assume xAllParticipantsInB(xid, B);
-  }
-}
-
-yield procedure {:layer 8}
-Coordinator_VoteYes (xid: Xid, mid: Mid, {:linear_in} pair: One Pair)
-refines atomic_Coordinator_VoteYes;
-requires call YieldInv_8();
-requires call YieldUndecidedOrCommitted_8(xid, mid, pair);
-{
-  var commit : bool;
-  var i : Mid;
-  var {:layer 8} snapshot: GState;
-
-  call {:layer 8} snapshot := Copy(state);
-  call {:layer 8} Lemma_add_to_set(B->val, pair->val);
-  call {:layer 8} Lemma_all_in_set(B->val, xid);
-  call commit := StateUpdateOnVoteYes(xid, mid, pair);
-  call {:layer 8} Lemma_all_in_set(B->val, xid);
-
-  if (commit)
-  {
-    assert {:layer 8} xUndecidedOrCommitted(snapshot[xid]);
-    assert {:layer 8} xUndecidedOrCommitted(state[xid]);
+    call votes, vrs' := voting_loop_yield_procedure(xid->val, vrs', n);
+    
     i := 1;
-    while (i <= numParticipants)
-    invariant {:layer 8} 1 <= i && i <= numParticipants + 1;
-    invariant {:layer 8} Inv_8(state, B, votes);
-    invariant {:layer 8} ExistsMonotoneExtension(snapshot, state, xid);
+    while (i <= n)
+    invariant {:layer 1} (forall {:pool "J"} j:int :: {:add_to_pool "J", j} 1 <= j && j < i ==> (d == COMMIT() ==> (votes[j] == YES())));
     {
-      async call {:sync} Participant_Commit(xid, i);
-      i := i + 1;
+        if (votes[i] == NO())
+        {
+            d := ABORT();
+        }
+        i := i+1;
     }
-  }
 
-  assert {:layer 8} {:add_to_pool "A", state[xid]} true;
+    call finalize_loop_yield_procedure(d, xid, vrs');
+
+    if (d == COMMIT())
+    {
+        par LockedNoConflicts() | CommittedSubsetLocked() |  XidNotInCommitted(xid) | XidInLocked(xid);
+
+        assume {:add_to_pool "J", 1} true;
+
+        call add_to_committed_transactions_procedure(xid);
+    }
 }
 
-left action {:layer 9} atomic_Coordinator_VoteNo (xid: Xid, mid: Mid, {:linear_in} pair: One Pair)
-modifies state;
+yield right procedure {:layer 1} voting_loop_yield_procedure(xid: TransactionId, {:linear_in} vrs: Set VoteRequest, i: int) returns (votes: [ReplicaId]Vote, {:linear} vrs': Set VoteRequest)
+requires {:layer 1} vrs == Set((lambda vr:VoteRequest :: vr->xid == xid && 1 <= vr->rid && vr->rid < i+1));
+ensures {:layer 1} (forall j:int :: 1 <= j && j < i+1 && votes[j] == YES() ==> Set_Contains(locked_transactions[j], xid));
+ensures {:layer 1} vrs' ==Set((lambda vr:VoteRequest :: vr->xid == xid && 1 <= vr->rid && vr->rid < i+1));
+preserves call LockedNoConflicts();
+preserves call CommittedSubsetLocked();
+ensures {:layer 1} (forall j:int :: 1 <= j && j < n+1 ==> IsSubset(old(locked_transactions)[j]->val, locked_transactions[j]->val));
+ensures {:layer 1} (forall j:int :: 1 <= j && j < i+1 ==> votes[j] != NONE());
+modifies locked_transactions;
 {
-  var {:pool "A"} next_state_xid: XState;
-  assert Set_IsDisjoint(perm(xid), UnallocatedXids);
-  assert pair(xid, mid, pair->val);
-  assert {:add_to_pool "A", state[xid]} xUndecidedOrAborted(state[xid]);
-  assume {:add_to_pool "A", next_state_xid} xConsistentExtension(state[xid], next_state_xid);
-  state[xid] := next_state_xid;
-  assume xUndecidedOrAborted(state[xid]);
+    var {:linear} vr: One VoteRequest;
+    var out: Vote;
+
+    vrs' := vrs;
+    if (1 <= i)
+    {
+        call vr := One_Get(vrs', VoteRequest(xid, i));
+        par votes, vrs' := voting_loop_yield_procedure(xid, vrs', i-1) |  out := voting_procedure(vr);
+        votes[i] := out;
+        call One_Put(vrs', vr);
+    }
 }
 
-yield procedure {:layer 8}
-Coordinator_VoteNo (xid: Xid, mid: Mid, {:linear_in} pair: One Pair)
-refines atomic_Coordinator_VoteNo;
-requires call YieldAborted_8(xid, mid, pair);
+yield left procedure {:layer 1} finalize_loop_yield_procedure(d: Decision, {:linear} xid: One TransactionId, {:linear_in} vrs: Set VoteRequest)
+requires {:layer 1} vrs == allVoteRequests(xid->val);
+requires {:layer 1}  (forall j:int :: {:add_to_pool "J", j} d == COMMIT() &&  1 <= j && j < n+1 ==> Set_Contains(locked_transactions[j], xid->val));
+ensures {:layer 1}  (forall j:int :: d == COMMIT() && 1 <=j && j < n+1 ==> Set_Contains(locked_transactions[j], xid->val));
+preserves call LockedNoConflicts();
+preserves call CommittedSubsetLocked();
+requires {:layer 1} !Set_Contains(committed_transactions, xid->val);
+ensures {:layer 1} (forall j:int, xid0 : TransactionId :: 1 <= j && j < n+1 && xid0 != xid->val && Set_Contains(old(locked_transactions)[j], xid0) ==> Set_Contains(locked_transactions[j], xid0));
+modifies locked_transactions;
 {
-  var abort : bool;
-  var i : int;
-  var {:layer 8} snapshot: GState;
+    var i: int;
+    var {:linear} vr: One VoteRequest;
+    var {:linear} vrs': Set VoteRequest;
 
-  call {:layer 8} snapshot := Copy(state);
-  call abort := StateUpdateOnVoteNo(xid, mid);
-
-  if (abort)
-  {
+    vrs' := vrs;
     i := 1;
-    while (i <= numParticipants)
-    invariant {:layer 8} 1 <= i && i <= numParticipants + 1;
-    invariant {:layer 8} Aborted(state[xid][CoordinatorMid]);
-    invariant {:layer 8} xUndecidedOrAborted(state[xid]);
-    invariant {:layer 8} ExistsMonotoneExtension(snapshot, state, xid);
+
+    while (i <= n)
+    invariant {:layer 1} (forall j:int :: d == COMMIT() && 1 <= j && j < i ==> Set_Contains(locked_transactions[j], xid->val));
+    invariant {:layer 1} (forall j:int :: d == COMMIT() && (i <= j) && (j < n+1)  ==> Set_Contains(locked_transactions[j], xid->val));
+    invariant {:layer 1} vrs' == remainingVoteRequests(xid->val, i);
+    invariant {:layer 1} (forall  j:int,  xid1: TransactionId, xid2: TransactionId :: (1 <= j && j < n+1 && xid1 != xid2 && Set_Contains(locked_transactions[j], xid1) && Set_Contains(locked_transactions[j], xid2)) ==> !Conflict[xid1][xid2]);
+    invariant {:layer 1} (forall j:int, xid0: TransactionId ::  1 <= j && j < n+1 && Set_Contains(committed_transactions, xid0) ==> Set_Contains(locked_transactions[j], xid0));
+    invariant {:layer 1} !Set_Contains(committed_transactions, xid->val);
+    invariant {:layer 1} (forall j:int, xid0 : TransactionId :: 1 <= j && j < n+1 && xid0 != xid->val && Set_Contains(old(locked_transactions)[j], xid0) ==> Set_Contains(locked_transactions[j], xid0));
     {
-      async call {:sync} Participant_Abort(xid, i);
-      i := i + 1;
+        call vr := One_Get(vrs', VoteRequest(xid->val, i));
+        async call {:sync} finalize_procedure(d, vr);
+        i := i + 1;
     }
-  }
-
-  assert {:layer 8} {:add_to_pool "A", state[xid]} true;
 }
 
-// ---------------------------------------------------------------------------
-
-yield procedure {:layer 7} SetParticipantAborted (xid: Xid, mid: Mid, {:linear} pair: One Pair);
-refines atomic_SetParticipantAborted;
-
-yield procedure {:layer 7} StateUpdateOnVoteYes (xid: Xid, mid: Mid, {:linear_in} pair: One Pair) returns (commit : bool);
-refines atomic_StateUpdateOnVoteYes;
-
-yield procedure {:layer 7} StateUpdateOnVoteNo (xid: Xid, mid: Mid) returns (abort : bool);
-refines atomic_StateUpdateOnVoteNo;
-
-yield procedure {:layer 7} Participant_Commit (xid : Xid, mid : Mid);
-refines atomic_Participant_Commit;
-
-yield procedure {:layer 7} Participant_Abort (xid : Xid, mid : Mid);
-refines atomic_Participant_Abort;
-
-atomic action {:layer 8,9} atomic_SetParticipantAborted (xid: Xid, mid: Mid, {:linear} pair: One Pair)
-modifies state;
+right action {:layer 1, 1} voting_action ( {:linear} vr: One VoteRequest) returns (result : Vote)
 {
-  assert pair(xid, mid, pair->val);
-  assert xUndecidedOrAborted(state[xid]);
-  state[xid][mid] := ABORTED();
+    if (*)
+    {
+        result := NO();
+    }
+    else
+    {
+        if (noConflicts(locked_transactions[vr->val->rid], vr->val->xid))
+        {
+            locked_transactions[vr->val->rid] := Set_Add(locked_transactions[vr->val->rid], vr->val->xid);
+            result := YES();
+        }
+        else
+        {
+            result := NO();
+        }
+    }
 }
+yield procedure {:layer 0} voting_procedure ({:linear} vr: One VoteRequest) returns (result : Vote);
+refines voting_action;
 
-atomic action {:layer 8} atomic_StateUpdateOnVoteYes (xid: Xid, mid: Mid, {:linear_in} pair: One Pair) returns (commit : bool)
-modifies votes, state, B;
+left action {:layer 1, 1} finalize_action (d: Decision, {:linear} vr: One VoteRequest)
 {
-  assert Set_IsDisjoint(perm(xid), UnallocatedXids);
-  assert VotesEqCoordinatorState(votes, state, xid);
-  call One_Put(B, pair);
-  if (votes[xid] == -1) {
-    commit := false;
-  } else {
-    votes[xid] := votes[xid] + 1;
-    commit := (votes[xid] == numParticipants);
-    state[xid][CoordinatorMid] := (if commit then COMMITTED() else state[xid][CoordinatorMid]);
-  }
+    if (d != COMMIT())
+    {
+        locked_transactions[vr->val->rid] := Set_Remove(locked_transactions[vr->val->rid], vr->val->xid);
+    }
 }
+yield procedure {:layer 0} finalize_procedure (d: Decision, {:linear} vr: One VoteRequest);
+refines finalize_action;
 
-atomic action {:layer 8} atomic_StateUpdateOnVoteNo (xid: Xid, mid: Mid) returns (abort : bool)
-modifies votes, state;
+
+atomic action {:layer 1, 1} add_to_committed_transactions({:linear} xid: One TransactionId)
 {
-  assert Set_IsDisjoint(perm(xid), UnallocatedXids);
-  assert !Committed(state[xid][CoordinatorMid]);
-  abort := (votes[xid] != -1);
-  votes[xid] := -1;
-  state[xid][CoordinatorMid] := (if abort then ABORTED() else state[xid][CoordinatorMid]);
+    assert (forall xid0: TransactionId :: Set_Contains(committed_transactions, xid0) ==> !Conflict[xid0][xid->val]);
+    committed_transactions := Set_Add(committed_transactions, xid->val);
 }
+yield procedure {:layer 0} add_to_committed_transactions_procedure ({:linear} xid: One TransactionId);
+refines add_to_committed_transactions;
 
-// ---------------------------------------------------------------------------
+yield invariant {:layer 1} LockedNoConflicts();
+invariant {:layer 1} (forall  {:pool "J"} j:int, xid1: TransactionId, xid2: TransactionId :: {:add_to_pool "J", j} (1 <= j && j < n+1 && xid1 != xid2 && Set_Contains(locked_transactions[j], xid1) && Set_Contains(locked_transactions[j], xid2)) ==> !Conflict[xid1][xid2]);
 
-left action {:layer 8} atomic_Participant_Commit (xid : Xid, mid : Mid)
-modifies state;
-{
-  assert participantMid(mid);
-  assert xUndecidedOrCommitted(state[xid]);
-  assert Committed(state[xid][CoordinatorMid]);
-  state[xid][mid] := COMMITTED();
-}
+yield invariant {:layer 1} CommittedSubsetLocked();
+invariant {:layer 1} (forall {:pool "J"} j:int, xid0: TransactionId :: {:add_to_pool "J", j} 1 <= j && j < n+1 && Set_Contains(committed_transactions, xid0) ==> Set_Contains(locked_transactions[j], xid0));
 
-left action {:layer 8} atomic_Participant_Abort (xid : Xid, mid : Mid)
-modifies state;
-{
-  assert participantMid(mid);
-  assert xUndecidedOrAborted(state[xid]);
-  assert Aborted(state[xid][CoordinatorMid]);
-  state[xid][mid] := ABORTED();
-}
+yield invariant {:layer 1} XidInLocked({:linear} xid: One TransactionId);
+invariant (forall {:pool "J"} j:int :: {:add_to_pool "J", j} 1 <= j && j < n+1 ==> Set_Contains(locked_transactions[j], xid->val));
 
-// ###########################################################################
-// Linear variable allocation
-
-atomic action {:layer 8,10} atomic_AllocateXid () returns (xid: Xid, {:linear} pairs: Set Pair)
-modifies UnallocatedXids;
-{
-  assume state[xid] == (lambda j: Mid :: UNDECIDED());
-  pairs := perm(xid);
-  assume Set_IsSubset(pairs, UnallocatedXids);
-  call Set_Split(UnallocatedXids, pairs);
-}
-yield procedure {:layer 7} AllocateXid () returns (xid: Xid, {:linear} pairs: Set Pair);
-refines atomic_AllocateXid;
-
-// ############################################################################
-// Lemmas about cardinality
-
-function card(pairs: [Pair]bool, xid: Xid) : int;
-
-pure procedure Lemma_add_to_set (set: [Pair]bool, pair: Pair);
-requires participantMid(pair->mid);
-requires !set[pair];
-ensures (forall xid: Xid :: card(set[pair := true], xid) == (if xid == pair->xid then card(set, xid) + 1 else card(set, xid)));
-
-pure procedure Lemma_all_in_set (set: [Pair]bool, xid: Xid);
-requires SetInv(set);
-ensures card(set, xid) >= numParticipants ==> (forall mid: Mid :: participantMid(mid) ==> set[Pair(xid, mid)]);
+yield invariant {:layer 1} XidNotInCommitted({:linear} xid: One TransactionId);
+invariant !Set_Contains(committed_transactions, xid->val);
+ 
